1) Added new features:    a) functions in output are a superset of functions in input, which can be in       a different order;    b) mapping function names between inputs and outputs         main -> softbound_pseudo_main         other-user-defined func -> softbound_func         some system func -> unchanged, say printf, which does not have           mem effects         other system func of mem effects -> softbounf_func         ...    c) an ad-hoc validator to check if the output symbolic mem state is a       "superset" of the input smem in terms of some axioms. These axioms       should be admissible from the memory model;
   Added testcases.

2) a code structure that works for both Emacs and OcaIDE.



git-svn-id: https://webdav.seas.upenn.edu/svn/sol/vol@2813 eef5ea85-cc2e-0410-bd84-0fae1f012da8

src/Interpreter/main.ml
@@ -6,47 +6,47 @@ open Llvm_executionengine
 open Trace
 
 let interInsnLoop (s0:LLVMopsem.coq_State) (tr0:trace) : (LLVMopsem.coq_State*trace) option =
-	
-	let s = ref s0 in
-	let n = ref 0 in
-	
-	while not (LLVMopsem.ds_isFinialState !s) do
-  	(if !Globalstates.debug then (eprintf "n=%d\n" !n;	 flush_all()));		
-		match interInsn !s with
+  
+  let s = ref s0 in
+  let n = ref 0 in
+  
+  while not (LLVMopsem.ds_isFinialState !s) do
+    (if !Globalstates.debug then (eprintf "n=%d\n" !n;   flush_all()));    
+    match interInsn !s with
     | Some (s', _) ->
-			begin 
-			  s := s';
-			  n := !n + 1
-			end 
+      begin 
+        s := s';
+        n := !n + 1
+      end 
     | None -> failwith "Stuck!" 
-	done;
-	
-	Some (!s, Coq_trace_nil)
-	
+  done;
+  
+  Some (!s, Coq_trace_nil)
+  
 let rec interInsnStar (s:LLVMopsem.coq_State) (tr:trace) (n:int) : (LLVMopsem.coq_State*trace) option =
-	if (LLVMopsem.ds_isFinialState s) 
-	then 
-		begin
-			(if !Globalstates.debug then (eprintf "Done!\n";flush_all()));
-			Some (s, tr)
-    end			
-	else
-		if n > 0 
-		then
-	    begin
-			(if !Globalstates.debug then (eprintf "n=%d\n" n;	 flush_all()));		
-			match interInsn s with
+  if (LLVMopsem.ds_isFinialState s) 
+  then 
+    begin
+      (if !Globalstates.debug then (eprintf "Done!\n";flush_all()));
+      Some (s, tr)
+    end      
+  else
+    if n > 0 
+    then
+      begin
+      (if !Globalstates.debug then (eprintf "n=%d\n" n;   flush_all()));    
+      match interInsn s with
       | Some (s', tr') -> interInsnStar s' (trace_app tr tr') (n-1)  
       | None ->
-				eprintf "Stuck!\n";flush_all(); 
-				None
-			end
-		else 
-			begin
-				eprintf "Time up!\n";flush_all();
-				Some (s, tr)
-      end				
-			
+        eprintf "Stuck!\n";flush_all(); 
+        None
+      end
+    else 
+      begin
+        eprintf "Time up!\n";flush_all();
+        Some (s, tr)
+      end        
+      
 let main in_filename argv =
 
         let ic = global_context () in
@@ -63,17 +63,17 @@ let main in_filename argv =
         let li = ExecutionEngine.create_interpreter imp in
 
         let print() = Array.iter print_endline argv in
-				
-				if !Globalstates.debug then 
-					(eprintf "main runs with arguments: \n"; print(); flush_all());
+        
+        if !Globalstates.debug then 
+          (eprintf "main runs with arguments: \n"; print(); flush_all());
 
-				let gargvs = (GenericValue.of_int (Llvm.integer_type ic 32) (Array.length argv))::
-				              ExecutionEngine.to_argv argv ic li::
-				              [] in
+        let gargvs = (GenericValue.of_int (Llvm.integer_type ic 32) (Array.length argv))::
+                      ExecutionEngine.to_argv argv ic li::
+                      [] in
 
         (* FIXME: We need to call ctors/dtors before/after execution *)
-				(* Do we also need to formalize them in Coq? They are implemented by*)
-				(* llvm.global_ctors/llvm.global_dtors. Are they target-independent? *)
+        (* Do we also need to formalize them in Coq? They are implemented by*)
+        (* llvm.global_ctors/llvm.global_dtors. Are they target-independent? *)
         ExecutionEngine.run_static_ctors li;
 
         (match LLVMopsem.ds_genInitState (coqim::[]) "@main" gargvs (li, im) with
@@ -83,33 +83,33 @@ let main in_filename argv =
               | None -> () )
           | None -> () );
         
-			  SlotTracker.dispose ist;
+        SlotTracker.dispose ist;
         ExecutionEngine.dispose li
 
 let _ = let len = Array.length Sys.argv in
-	
-	      if len < 1 then
-	        failwith "# of argv is 0";
-													
-				let idx = ref 1 in				
-				let set_flags = fun _ ->
-  				let finished = ref false in	
-				  while (not !finished) && (!idx < len) do
-						let arg = Array.get Sys.argv !idx in
-						
-						if arg = "-d" then 
-							Globalstates.debug := true;
-					
-					  if String.get arg 0 != '-' 
-						then
-							finished := true
-						else	
-						  idx := !idx + 1 		  							
-					done in
-																
+  
+        if len < 1 then
+          failwith "# of argv is 0";
+                          
+        let idx = ref 1 in        
+        let set_flags = fun _ ->
+          let finished = ref false in  
+          while (not !finished) && (!idx < len) do
+            let arg = Array.get Sys.argv !idx in
+            
+            if arg = "-d" then 
+              Globalstates.debug := true;
+          
+            if String.get arg 0 != '-' 
+            then
+              finished := true
+            else  
+              idx := !idx + 1                     
+          done in
+                                
         set_flags ();
-																																
-				if !idx < len then
-					main (Array.get Sys.argv !idx) (Array.sub Sys.argv !idx (len - !idx))
-				else
-					main "Input.bc" (Array.make 1 "")		
+                                                                
+        if !idx < len then
+          main (Array.get Sys.argv !idx) (Array.sub Sys.argv !idx (len - !idx))
+        else
+          main "Input.bc" (Array.make 1 "")    
