src/TV/sub_tv.v
@@ -35,7 +35,10 @@ sumbool2bool _ _ (sstate_sub_dec (se_cmds sstate_init nbs1) (se_cmds sstate_init
 (* Realized to check if two function names are matched. For example,
  * in Softbound, 'test' in the original program matches 'softbound_test'.
 *)
-Axiom tv_fid : id -> id -> bool.
+Axiom rename_fid : id -> id.
+
+Definition tv_fid (fid1 fid2:id) := 
+  sumbool2bool _ _ (id_dec (rename_fid fid1) fid2).
 
 Axiom tv_fid_injective1 : forall fid1 fid2 fid1' fid2',
   fid1 = fid2 -> tv_fid fid1 fid1' -> tv_fid fid2 fid2' -> fid1' = fid2'.
@@ -122,34 +125,286 @@ match (f1, f2) with
   tv_fheader fh1 fh2 && tv_blocks lb1 lb2
 end.
 
-Fixpoint tv_products (Ps1 Ps2:products):=
-match (Ps1, Ps2) with
-| (nil, nil) => true
-| (product_fdec f1::Ps1', product_fdec f2::Ps2') => 
-  sumbool2bool _ _ (fdec_dec f1 f2) &&
-  tv_products Ps1' Ps2'
-| (product_fdef f1::Ps1', product_fdef f2::Ps2') => 
-  tv_fdef f1 f2 && tv_products Ps1' Ps2'
-| (product_gvar gvar1::Ps1', product_gvar gvar2::Ps2') => 
-  sumbool2bool _ _ (gvar_dec gvar1 gvar2) &&
-  tv_products Ps1' Ps2'
-| _ => false
+Definition tv_fdec (f1 f2:fdec) :=
+match (f1, f2) with
+| (fdec_intro fh1, fdec_intro fh2) => tv_fheader fh1 fh2
 end.
 
-Definition tv_module (m1 m2:module) :=
-match (m1, m2) with
-| (module_intro los1 nts1 Ps1, module_intro los2 nts2 Ps2) =>
-  sumbool2bool _ _ (layouts_dec los1 los2) &&
-  sumbool2bool _ _ (namedts_dec nts1 nts2) &&
-  tv_products Ps1 Ps2
+Fixpoint lookupGvarViaIDFromProducts (lp:products) (i:id) : option gvar :=
+match lp with
+| nil => None
+| (product_gvar gv)::lp' => 
+    if (eq_dec (getGvarID gv) i) then Some gv
+    else lookupGvarViaIDFromProducts lp' i
+| _::lp' => lookupGvarViaIDFromProducts lp' i
 end.
 
-Fixpoint tv_system (S1 S2:system) :=
-match (S1, S2) with
-| (nil, nil) => true
-| (m1::S1', m2::S2') => tv_module m1 m2 && tv_system S1' S2'
-| _ => false
-end.
+Definition products_sub (Ps1 Ps2:products) := forall id1, 
+  In id1 (getProductsIDs Ps1) ->
+  (forall fdec1,
+    lookupFdecViaIDFromProducts Ps1 id1 = Some fdec1 ->
+    exists fdec2,
+      lookupFdecViaIDFromProducts Ps2 (rename_fid id1) = Some fdec2 /\ 
+      tv_fdec fdec1 fdec2 = true)
+  /\
+  (forall fdef1,
+    lookupFdefViaIDFromProducts Ps1 id1 = Some fdef1 ->
+    exists fdef2,
+      lookupFdefViaIDFromProducts Ps2 (rename_fid id1) = Some fdef2 /\ 
+      tv_fdef fdef1 fdef2 = true)
+  /\
+  (forall gv1,
+    lookupGvarViaIDFromProducts Ps1 id1 = Some gv1 ->
+    exists gv2,
+      lookupGvarViaIDFromProducts Ps2 id1 = Some gv2 /\ 
+      sumbool2bool _ _ (gvar_dec gv1 gv2) = true).
+
+(*
+Lemma lookupAL_app1 : forall X (lc1:list (atom*X)) lc2 i,
+  i `in` dom lc1 ->
+  lookupAL X lc1 i = lookupAL X (lc1++lc2) i.
+Proof.
+  induction lc1; intros lc2 i Hi_in_lc1.
+    fsetdec.
+    destruct a as (id, elt); simpl in *.
+    destruct (@eq_dec atom (EqDec_eq_of_EqDec atom EqDec_atom) i id); auto.
+      apply IHlc1. fsetdec.
+Qed.    
+
+Lemma lookupAL_app2 : forall X lc1 (lc2:list (atom*X)) i,
+  i `notin` dom lc1 ->
+  lookupAL X lc2 i = lookupAL X (lc1++lc2) i.
+Proof.
+  induction lc1; intros lc2 i Hi_notin_lc1; auto.
+    destruct a as (id, elt); simpl in *.
+    destruct (@eq_dec atom (EqDec_eq_of_EqDec atom EqDec_atom) i id); subst; eauto.
+      fsetdec.
+Qed.    
+*)
+
+Lemma products_sub_app1 : forall Ps1 Ps2 Ps,
+  products_sub Ps1 Ps -> 
+  products_sub Ps2 Ps ->
+  products_sub (Ps1++Ps2) Ps.
+Proof.
+  intros Ps1 Ps2 Ps HPs1_sub_Ps HPs2_sub_Ps.
+  intros i i_in_Ps12.
+(*
+  simpl_env in i_in_lc12.
+  apply in_dom_app_inv in i_in_lc12.
+  assert (i `in`  dom lc1 \/ i `notin` dom lc1) as i_in_lc1_dec. fsetdec.
+  destruct i_in_lc1_dec as [i_in_lc1 | i_notin_lc1].
+    rewrite <- Hlc1_sub_lc; auto.
+    rewrite <- lookupAL_app1; auto.
+
+    destruct i_in_lc12 as [i_in_lc1 | i_in_lc2].
+      fsetdec.
+      rewrite <- lookupAL_app2; auto.
+*)
+Admitted.
+
+(*
+Lemma lookupALs_tail : forall X l2b l2b' l0,
+  l0 `notin` dom l2b ->
+  lookupAL X (l2b++l2b') l0 = lookupAL _ l2b' l0.
+Proof.
+  intros.
+  induction l2b; auto.
+    destruct a. simpl in *.
+    destruct (@eq_dec atom (@EqDec_eq_of_EqDec atom EqDec_atom) l0 a); subst; auto.
+      fsetdec.
+Qed.
+*)
+
+Lemma products_sub_app2 : forall Ps1 Ps2 Ps,
+  products_sub Ps1 Ps -> 
+  NoDup (getProductsIDs (Ps1++Ps2)) ->
+  ~ products_sub Ps2 Ps ->
+  ~ products_sub (Ps1++Ps2) Ps.
+Admitted.
+(*
+Proof.
+  intros X lc1 lc2 lc Hlc1_sub_lc Hdisj Hlc2_nsub_lc Hlc12_sub_lc.
+  apply Hlc2_nsub_lc.
+  intros i i_in_lc2.
+    assert (i `notin` dom lc1) as i_notin_lc1. solve_uniq.
+    assert (i `in` dom (lc1++lc2)) as i_in_lc12. simpl_env. fsetdec.
+    apply Hlc12_sub_lc in i_in_lc12.
+    erewrite lookupALs_tail in i_in_lc12; eauto.
+Qed.
+*)
+
+Lemma products_sub_dec: forall Ps1 Ps2, 
+  NoDup (getProductsIDs Ps1) ->
+  {products_sub Ps1 Ps2} + {~products_sub Ps1 Ps2}.
+Proof.
+  induction Ps1; intros Ps2 Huniq.
+    left. intros id1 Hindom. 
+    inversion Hindom.
+
+    simpl in Huniq.
+    rewrite_env (nil ++ getProductID a :: getProductsIDs Ps1) in Huniq.
+    assert (Hnotindom:=Huniq).
+    apply NoDup_remove_2 in Hnotindom.
+    assert (Huniq':=Huniq).
+    apply NoDup_remove_1 in Huniq'.
+    simpl_env in *.
+    destruct a as [g1 | f1 | f1].
+    Case "gvar".
+      remember (lookupGvarViaIDFromProducts Ps2 (getGvarID g1)) as Lookup.
+      destruct Lookup as [g2 | ].
+      SCase "gid in Ps2".
+        destruct (gvar_dec g1 g2); subst.
+        SSCase "g1 = g2".
+          assert (products_sub [product_gvar g2] Ps2) as Hg2_sub_Ps2.
+            intros i Hi_in_dom. simpl. 
+            repeat split; try solve [intros a Hlookup; inversion Hlookup].
+            intros gv1 Hlookup.
+            destruct (@eq_dec id (EqDec_eq_of_EqDec id EqDec_atom) (getGvarID g2) i); inversion Hlookup; subst.
+              exists gv1. split; auto.
+              destruct (gvar_dec gv1 gv1); simpl; auto.
+          destruct (@IHPs1 Ps2 Huniq') as [HPs1_sub_Ps2 | HPs1_nsub_Ps2].
+            left. apply products_sub_app1; auto.
+            right. apply products_sub_app2; auto.
+          
+        SSCase "g1 <> g2".
+          right. intro J.
+          assert (In (getGvarID g1) (getProductsIDs ([product_gvar g1]++Ps1))) 
+            as Hindom. 
+            simpl. auto.
+          assert (H:=@J (getGvarID g1) Hindom). simpl in H.
+          destruct H as [_ [_ H3]].
+          destruct (@eq_dec id (EqDec_eq_of_EqDec id EqDec_atom) (getGvarID g1) (getGvarID g1)) as [e | n']; try solve [contradict n'; auto].
+          destruct (@H3 g1) as [gv2 [J1 J2]]; auto.
+          rewrite <- HeqLookup in J1. inversion J1; subst.
+          destruct (gvar_dec g1 gv2); subst; auto.
+            simpl in J2. inversion J2.
+
+      SCase "gid notin Ps2".
+        right. intro J.
+        assert (In (getGvarID g1) (getProductsIDs ([product_gvar g1]++Ps1))) 
+          as Hindom. 
+          simpl. auto.
+        assert (H:=@J (getGvarID g1) Hindom). simpl in H.
+        destruct H as [H1 [H2 H3]].
+        destruct (@eq_dec id (EqDec_eq_of_EqDec id EqDec_atom) (getGvarID g1) (getGvarID g1)) as [e | n']; try solve [contradict n'; auto].
+        destruct (@H3 g1) as [gv2 [J1 J2]]; auto.       
+        rewrite <- HeqLookup in J1. inversion J1.
+        
+    Case "fdec".
+      remember (lookupFdecViaIDFromProducts Ps2 (rename_fid (getFdecID f1))) as Lookup.
+      destruct Lookup as [f2 | ].
+      SCase "fid in Ps2".
+        remember (tv_fdec f1 f2) as R.
+        destruct R; subst.
+        SSCase "f1 = f2".
+          assert (products_sub [product_fdec f1] Ps2) as Hf2_sub_Ps2.
+            intros i Hi_in_dom. simpl. 
+            repeat split; try solve [intros a Hlookup; inversion Hlookup].
+            intros fdec1 Hlookup.
+            destruct (@eq_dec id (EqDec_eq_of_EqDec id EqDec_atom) (getFdecID f1) i); inversion Hlookup; subst.
+              exists f2. split; auto.
+          destruct (@IHPs1 Ps2 Huniq') as [HPs1_sub_Ps2 | HPs1_nsub_Ps2].
+            left. apply products_sub_app1; auto.
+            right. apply products_sub_app2; auto.
+          
+        SSCase "f1 <> f2".
+          right. intro J.
+          assert (In (getFdecID f1) (getProductsIDs ([product_fdec f1]++Ps1))) 
+            as Hindom. 
+            simpl. auto.
+          assert (H:=@J (getFdecID f1) Hindom). simpl in H.
+          destruct H as [H1 _].
+          destruct (@eq_dec id (EqDec_eq_of_EqDec id EqDec_atom) (getFdecID f1) (getFdecID f1)) as [e | n']; try solve [contradict n'; auto].
+          destruct (@H1 f1) as [fdec2 [J1 J2]]; auto.
+          rewrite <- HeqLookup in J1. inversion J1; subst.
+          rewrite J2 in HeqR. inversion HeqR.
+
+      SCase "fid notin Ps2".
+        right. intro J.
+        assert (In (getFdecID f1) (getProductsIDs ([product_fdec f1]++Ps1))) 
+          as Hindom. 
+          simpl. auto.
+        assert (H:=@J (getFdecID f1) Hindom). simpl in H.
+        destruct H as [H1 [H2 H3]].
+        destruct (@eq_dec id (EqDec_eq_of_EqDec id EqDec_atom) (getFdecID f1) (getFdecID f1)) as [e | n']; try solve [contradict n'; auto].
+        destruct (@H1 f1) as [fdec2 [J1 J2]]; auto.       
+        rewrite <- HeqLookup in J1. inversion J1.
+
+    Case "fdef".
+      remember (lookupFdefViaIDFromProducts Ps2 (rename_fid (getFdefID f1))) as Lookup.
+      destruct Lookup as [f2 | ].
+      SCase "fid in Ps2".
+        remember (tv_fdef f1 f2) as R.
+        destruct R; subst.
+        SSCase "f1 = f2".
+          assert (products_sub [product_fdef f1] Ps2) as Hf2_sub_Ps2.
+            intros i Hi_in_dom. simpl. 
+            repeat split; try solve [intros a Hlookup; inversion Hlookup].
+            intros fdef1 Hlookup.
+            destruct (@eq_dec id (EqDec_eq_of_EqDec id EqDec_atom) (getFdefID f1) i); inversion Hlookup; subst.
+              exists f2. split; auto.
+          destruct (@IHPs1 Ps2 Huniq') as [HPs1_sub_Ps2 | HPs1_nsub_Ps2].
+            left. apply products_sub_app1; auto.
+            right. apply products_sub_app2; auto.
+          
+        SSCase "f1 <> f2".
+          right. intro J.
+          assert (In (getFdefID f1) (getProductsIDs ([product_fdef f1]++Ps1))) 
+            as Hindom. 
+            simpl. auto.
+          assert (H:=@J (getFdefID f1) Hindom). simpl in H.
+          destruct H as [_ [H2 _]].
+          destruct (@eq_dec id (EqDec_eq_of_EqDec id EqDec_atom) (getFdefID f1) (getFdefID f1)) as [e | n']; try solve [contradict n'; auto].
+          destruct (@H2 f1) as [fdef2 [J1 J2]]; auto.
+          rewrite <- HeqLookup in J1. inversion J1; subst.
+          rewrite J2 in HeqR. inversion HeqR.
+
+      SCase "fid notin Ps2".
+        right. intro J.
+        assert (In (getFdefID f1) (getProductsIDs ([product_fdef f1]++Ps1))) 
+          as Hindom. 
+          simpl. auto.
+        assert (H:=@J (getFdefID f1) Hindom). simpl in H.
+        destruct H as [_ [H2 _]].
+        destruct (@eq_dec id (EqDec_eq_of_EqDec id EqDec_atom) (getFdefID f1) (getFdefID f1)) as [e | n']; try solve [contradict n'; auto].
+        destruct (@H2 f1) as [fdec2 [J1 J2]]; auto.       
+        rewrite <- HeqLookup in J1. inversion J1.
+Qed.
+
+Lemma tv_products: forall (Ps1 Ps2:products), NoDup (getProductsIDs Ps1) -> bool.
+Proof.
+  intros Ps1 Ps2 Huniq.
+  apply (sumbool2bool _ _ (products_sub_dec Ps1 Ps2 Huniq)).
+Defined.
+
+Lemma tv_module : forall (m1 m2:module), uniqModule m1 -> bool.
+Proof.
+  intros m1 m2 Huniq.
+  destruct m1 as [los1 nts1 Ps1].
+  destruct m2 as [los2 nts2 Ps2].
+  destruct Huniq as [_ [_ Huniq]].
+  apply (sumbool2bool _ _ (layouts_dec los1 los2) &&
+         sumbool2bool _ _ (namedts_dec nts1 nts2) &&
+         tv_products Ps1 Ps2 Huniq).
+Defined.
+
+Lemma tv_system : forall (S1 S2:system), uniqSystem S1 -> bool.
+Proof.
+  induction S1 as [ | m1 S1]; intros S2 Huniq.
+    destruct S2.
+      apply true.
+      apply false.
+
+    destruct S2 as [ | m2 S2].
+      apply false.
+
+      assert (uniqModule m1) as Huniq1.
+        inversion Huniq; auto.
+      assert (uniqSystem S1) as Huniq2.
+        inversion Huniq; auto.
+      apply (tv_module m1 m2 Huniq1 && IHS1 S2 Huniq2).
+Defined.
 
 Ltac sumbool_simpl :=
   repeat
